---
title: Reversal of formal series ğŸš§
---

```
{-# OPTIONS --guardedness --sized-types #-}
-- {-# OPTIONS --allow-unsolved-metas #-}

open import Preliminaries.Base hiding (_++_)
open import General.ProductRules

module Special.Reversal-ext
    (R : CommutativeRing)
    (Î£ : Set)
    (P : ProductRule R)
    where

open import Size
open import Preliminaries.List
open import Preliminaries.Algebra R
open import Preliminaries.PolyExpr R
    using (PolyExpr; con)
    renaming (subst to P-subst; âŸ¦_âŸ§_ to PâŸ¦_âŸ§_)

open import General.Series R Î£
open import General.Terms R renaming (_+_ to _[+]_; _*_ to _[*]_; _Â·_ to _[Â·]_) hiding (x; y; z; t)
open import General.Products R Î£
open import General.Automata R Î£ P
open import General.Reversal R Î£
open import General.ReversalEnd R Î£ P

open Product P
-- open Reversal P

open import Special.Polynomials R as P renaming (_â‰ˆ_ to _Pâ‰ˆ_)
open import Special.ProductRules R

private variable
    i : Size
    n : â„•
```

```
Î”Ê³Î”Ë¡ : Set
Î”Ê³Î”Ë¡ = âˆ€ a b Î± â†’ Î”Ê³ b â†‘ (Î”Ë¡ a â†‘ Î±) Pâ‰ˆ Î”Ë¡ a â†‘ (Î”Ê³ b â†‘ Î±)
```

```
module Assumptions (a b : Î£) where

    data aXb : Set where
        y : aXb
        ay : aXb
        yb : aXb
        ayb : aXb
        z : aXb
        az : aXb
        zb : aXb
        azb : aXb

    data aX : Set where
        y : aX
        ay : aX
        z : aX
        az : aX

    data Xb : Set where
        y : Xb
        yb : Xb
        z : Xb
        zb : Xb

    data ÎµXÎµ : Set where
        y : ÎµXÎµ
        z : ÎµXÎµ

    Îµâ†’a : Term ÎµXÎµ â†’ Term aX
    Îµâ†’a 0T = 0T
    Îµâ†’a (var y) = var y
    Îµâ†’a (var z) = var z
    Îµâ†’a (c [Â·] u) = c [Â·] Îµâ†’a u
    Îµâ†’a (u [+] v) = Îµâ†’a u [+] Îµâ†’a v
    Îµâ†’a (u [*] v) = Îµâ†’a u [*] Îµâ†’a v

    Îµâ†’b : Term ÎµXÎµ â†’ Term Xb
    Îµâ†’b 0T = 0T
    Îµâ†’b (var y) = var y
    Îµâ†’b (var z) = var z
    Îµâ†’b (c [Â·] u) = c [Â·] Îµâ†’b u
    Îµâ†’b (u [+] v) = Îµâ†’b u [+] Îµâ†’b v
    Îµâ†’b (u [*] v) = Îµâ†’b u [*] Îµâ†’b v

    aâ†’ab : Term aX â†’ Term aXb
    aâ†’ab 0T = 0T
    aâ†’ab (var y) = var y
    aâ†’ab (var ay) = var ay
    aâ†’ab (var z) = var z
    aâ†’ab (var az) = var az
    aâ†’ab (c [Â·] u) = c [Â·] aâ†’ab u
    aâ†’ab (u [+] v) = aâ†’ab u [+] aâ†’ab v
    aâ†’ab (u [*] v) = aâ†’ab u [*] aâ†’ab v

    bâ†’ab : Term Xb â†’ Term aXb
    bâ†’ab 0T = 0T
    bâ†’ab (var y) = var y
    bâ†’ab (var yb) = var yb
    bâ†’ab (var z) = var z
    bâ†’ab (var zb) = var zb
    bâ†’ab (c [Â·] u) = c [Â·] bâ†’ab u
    bâ†’ab (u [+] v) = bâ†’ab u [+] bâ†’ab v
    bâ†’ab (u [*] v) = bâ†’ab u [*] bâ†’ab v

    Î”Ë¡Îµ : Term ÎµXÎµ â†’ Term aX
    Î”Ë¡Îµ 0T = 0T
    Î”Ë¡Îµ (var y) = var ay
    Î”Ë¡Îµ (var z) = var az
    Î”Ë¡Îµ (c [Â·] Î³) = c [Â·] Î”Ë¡Îµ Î³
    Î”Ë¡Îµ (Î³ [+] Î´) = Î”Ë¡Îµ Î³ [+] Î”Ë¡Îµ Î´
    Î”Ë¡Îµ (Î³ [*] Î´) = [ P ]âŸ¨ Îµâ†’a Î³ , Î”Ë¡Îµ Î³ , Îµâ†’a Î´ , Î”Ë¡Îµ Î´ âŸ©

    Î”Ê³Îµ : Term ÎµXÎµ â†’ Term Xb
    Î”Ê³Îµ 0T = 0T
    Î”Ê³Îµ (var y) = var yb
    Î”Ê³Îµ (var z) = var zb
    Î”Ê³Îµ (c [Â·] Î³) = c [Â·] Î”Ê³Îµ Î³
    Î”Ê³Îµ (Î³ [+] Î´) = Î”Ê³Îµ Î³ [+] Î”Ê³Îµ Î´
    Î”Ê³Îµ (Î³ [*] Î´) = [ P ]âŸ¨ Îµâ†’b Î³ , Î”Ê³Îµ Î³ , Îµâ†’b Î´ , Î”Ê³Îµ Î´ âŸ©

    Î”Ë¡b : Term Xb â†’ Term aXb
    Î”Ë¡b 0T = 0T
    Î”Ë¡b (var y) = var ay
    Î”Ë¡b (var yb) = var ayb
    Î”Ë¡b (var z) = var az
    Î”Ë¡b (var zb) = var azb
    Î”Ë¡b (c [Â·] Î³) = c [Â·] Î”Ë¡b Î³
    Î”Ë¡b (Î³ [+] Î´) = Î”Ë¡b Î³ [+] Î”Ë¡b Î´
    Î”Ë¡b (Î³ [*] Î´) = [ P ]âŸ¨ bâ†’ab Î³ , Î”Ë¡b Î³ , bâ†’ab Î´ , Î”Ë¡b Î´ âŸ©

    Î”Ê³a : Term aX â†’ Term aXb
    Î”Ê³a 0T = 0T
    Î”Ê³a (var y) = var yb
    Î”Ê³a (var ay) = var ayb
    Î”Ê³a (var z) = var zb
    Î”Ê³a (var az) = var azb
    Î”Ê³a (c [Â·] Î³) = c [Â·] Î”Ê³a Î³
    Î”Ê³a (Î³ [+] Î´) = Î”Ê³a Î³ [+] Î”Ê³a Î´
    Î”Ê³a (Î³ [*] Î´) = [ P ]âŸ¨ aâ†’ab Î³ , Î”Ê³a Î³ , aâ†’ab Î´ , Î”Ê³a Î´ âŸ©
    
    -- t : Term ÎµXÎµ
    -- t = var y [*] var z

Î”Ê³Î”Ë¡-var : Set
Î”Ê³Î”Ë¡-var =
    âˆ€ a b â†’
    let open Assumptions a b in
    --------------------------
    Î”Ê³a (Î”Ë¡Îµ (var y [*] var z)) Pâ‰ˆ Î”Ë¡b (Î”Ê³Îµ (var y [*] var z))

Î”Ê³Î”Ë¡-varâ€² : Set
Î”Ê³Î”Ë¡-varâ€² =
    âˆ€ a b f g â†’
    -----------------------------------------------------------
    Î”Ê³ b â†‘ (Î”Ë¡ a â†‘ (var (Îµ x[ f ] Îµ) [*] var (Îµ x[ g ] Îµ))) Pâ‰ˆ
    Î”Ë¡ a â†‘ (Î”Ê³ b â†‘ (var (Îµ x[ f ] Îµ) [*] var (Îµ x[ g ] Îµ)))

module Test a b f g where

    open Assumptions a b

    ÏÎµ : Term ÎµXÎµ â†’ Term *X*
    ÏÎµ 0T = 0T
    ÏÎµ (var y) = var (Îµ x[ f ] Îµ)
    ÏÎµ (var z) = var (Îµ x[ g ] Îµ)
    ÏÎµ (c [Â·] Î³) = c [Â·] ÏÎµ Î³
    ÏÎµ (Î³ [+] Î´) = ÏÎµ Î³ [+] ÏÎµ Î´
    ÏÎµ (Î³ [*] Î´) = ÏÎµ Î³ [*] ÏÎµ Î´

    Ïa : Term aX â†’ Term *X*
    Ïa 0T = 0T
    Ïa (var y) = var (Îµ x[ f ] Îµ)
    Ïa (var ay) = var ((a âˆ· Îµ) x[ f ] Îµ)
    Ïa (var z) = var (Îµ x[ g ] Îµ)
    Ïa (var az) = var ((a âˆ· Îµ) x[ g ] Îµ)
    Ïa (c [Â·] Î³) = c [Â·] Ïa Î³
    Ïa (Î³ [+] Î´) = Ïa Î³ [+] Ïa Î´
    Ïa (Î³ [*] Î´) = Ïa Î³ [*] Ïa Î´

    Ïab : Term aXb â†’ Term *X*
    Ïab 0T = 0T
    Ïab (var y) = var (Îµ x[ f ] Îµ)
    Ïab (var ay) = var ((a âˆ· Îµ) x[ f ] Îµ)
    Ïab (var yb) = var (Îµ x[ f ] (b âˆ· Îµ))
    Ïab (var ayb) = var ((a âˆ· Îµ) x[ f ] (b âˆ· Îµ))
    Ïab (var z) = var (Îµ x[ g ] Îµ)
    Ïab (var az) = var ((a âˆ· Îµ) x[ g ] Îµ)
    Ïab (var zb) = var (Îµ x[ g ] (b âˆ· Îµ))
    Ïab (var azb) = var ((a âˆ· Îµ) x[ g ] (b âˆ· Îµ))
    Ïab (c [Â·] Î³) = c [Â·] Ïab Î³
    Ïab (Î³ [+] Î´) = Ïab Î³ [+] Ïab Î´
    Ïab (Î³ [*] Î´) = Ïab Î³ [*] Ïab Î´

    data aXbâ€² : *X* â†’ Set where
        y : aXbâ€² (Îµ x[ f ] Îµ)
        ay : aXbâ€² ((a âˆ· Îµ) x[ f ] Îµ)
        yb : aXbâ€² (Îµ x[ f ] (b âˆ· Îµ))
        ayb : aXbâ€² ((a âˆ· Îµ) x[ f ] (b âˆ· Îµ))
        z : aXbâ€² (Îµ x[ g ] Îµ)
        az : aXbâ€² ((a âˆ· Îµ) x[ g ] Îµ)
        zb : aXbâ€² (Îµ x[ g ] (b âˆ· Îµ))
        azb : aXbâ€² ((a âˆ· Îµ) x[ g ] (b âˆ· Îµ))

    -- must assume f âŸ¨ Îµ âŸ© â‰  g âŸ¨ Îµ âŸ©
    -- etc.

    aXbâ€²-inj : âˆ€ {x} (p q : aXbâ€² x) â†’ p â‰¡ q
    aXbâ€²-inj y y = {!   !}
    aXbâ€²-inj y z = {!   !}
    aXbâ€²-inj ay ay = {!   !}
    aXbâ€²-inj ay az = {!   !}
    aXbâ€²-inj yb yb = {!   !}
    aXbâ€²-inj yb zb = {!   !}
    aXbâ€²-inj ayb ayb = {!   !}
    aXbâ€²-inj ayb azb = {!   !}
    aXbâ€²-inj z y = {!   !}
    aXbâ€²-inj z z = {!   !}
    aXbâ€²-inj az ay = {!   !}
    aXbâ€²-inj az az = {!   !}
    aXbâ€²-inj zb yb = {!   !}
    aXbâ€²-inj zb zb = {!   !}
    aXbâ€²-inj azb ayb = {!   !}
    aXbâ€²-inj azb azb = {!   !}

    data Term-Prop (Var-Prop : *X* â†’ Set) : Term *X* â†’ Set where
        0T : Term-Prop Var-Prop 0T
        var : âˆ€ {x} (prop : Var-Prop x) â†’ Term-Prop Var-Prop (var x)
        _[Â·]_ : âˆ€ {u} c â†’ Term-Prop Var-Prop u â†’ Term-Prop Var-Prop (c [Â·] u)
        _[+]_ : âˆ€ {u v} â†’ Term-Prop Var-Prop u â†’ Term-Prop Var-Prop v â†’ Term-Prop Var-Prop (u [+] v)
        _[*]_ : âˆ€ {u v} â†’ Term-Prop Var-Prop u â†’ Term-Prop Var-Prop v â†’ Term-Prop Var-Prop (u [*] v)

    Term-Prop-inj : âˆ€ {Î±} (p q : Term-Prop aXbâ€² Î±) â†’ p â‰¡ q

    Term-Prop-inj 0T 0T = refl
    Term-Prop-inj (var px) (var qx) = {!   !}
    Term-Prop-inj (c [Â·] p) (.c [Â·] q) = {!   !}
    Term-Prop-inj (p [+] pâ‚) (q [+] qâ‚) = {!   !}
    Term-Prop-inj (p [*] pâ‚) (q [*] qâ‚) = {!   !}

    Ïab-inv : âˆ€ {Î±} â†’ Term-Prop aXbâ€² Î± â†’ Term aXb
    Ïab-inv 0T = 0T
    Ïab-inv (var y) = var {!   !}
    Ïab-inv (var ay) = {!   !}
    Ïab-inv (var yb) = {!   !}
    Ïab-inv (var ayb) = {!   !}
    Ïab-inv (var z) = {!   !}
    Ïab-inv (var az) = {!   !}
    Ïab-inv (var zb) = {!   !}
    Ïab-inv (var azb) = {!   !}
    Ïab-inv (c [Â·] Î±) = c [Â·] Ïab-inv Î±
    Ïab-inv (Î± [+] Î²) = Ïab-inv Î± [+] Ïab-inv Î²
    Ïab-inv (Î± [*] Î²) = Ïab-inv Î± [*] Ïab-inv Î²

    transferâ€² :
        âˆ€ {Î± Î² : Term *X*} â†’
        (pÎ± : Term-Prop aXbâ€² Î±) â†’
        (pÎ² : Term-Prop aXbâ€² Î²) â†’
        Î± Pâ‰ˆ Î² â†’
        -----------------------------
        Ïab-inv pÎ± Pâ‰ˆ Ïab-inv pÎ²

    transferâ€² pÎ± pÎ² â‰ˆ-refl = {!   !}
    transferâ€² pÎ± pÎ² (â‰ˆ-sym Î±â‰ˆÎ²) = {!   !}
    transferâ€² pÎ± pÎ² (â‰ˆ-trans Î±â‰ˆÎ² Î±â‰ˆÎ²â‚) = {!   !}
    transferâ€² pÎ± pÎ² (Â·-cong x Î±â‰ˆÎ²) = {!   !}
    transferâ€² pÎ± pÎ² (Â·-one _) = {!   !}
    transferâ€² pÎ± pÎ² (Â·-+-distrib c p q) = {!   !}
    transferâ€² pÎ± pÎ² (+-Â·-distrib p c d) = {!   !}
    transferâ€² pÎ± pÎ² (Â·-*-distrib c p q) = {!   !}
    transferâ€² pÎ± pÎ² (*-Â·-distrib c d p) = {!   !}
    transferâ€² pÎ± pÎ² (+-cong Î±â‰ˆÎ² Î±â‰ˆÎ²â‚) = {!   !}
    transferâ€² pÎ± pÎ² (+-zeroÊ³ _) = {!   !}
    transferâ€² pÎ± pÎ² (+-assoc p q r) = {!   !}
    transferâ€² pÎ± pÎ² (+-comm p q) = {!   !}
    transferâ€² pÎ± pÎ² (+-invÊ³ p) = {!   !}
    transferâ€² pÎ± pÎ² (*-cong Î±â‰ˆÎ² Î±â‰ˆÎ²â‚) = {!   !}
    transferâ€² pÎ± pÎ² (*-assoc p q r) = {!   !}
    transferâ€² pÎ± pÎ² (*-comm p q) = {!   !}
    transferâ€² pÎ± pÎ² (*-distribÊ³ p q r) = {!   !}

    transfer : âˆ€ (Î³ Î´ : Term aXb) â†’ Ïab Î³ Pâ‰ˆ Ïab Î´ â†’ Î³ Pâ‰ˆ Î´
    transfer = {!   !}


    ÏÎ”Ë¡Îµ-lem : 
        (Î³ : Term ÎµXÎµ) â†’
        ---------------------------
        Ïa (Î”Ë¡Îµ Î³) Pâ‰ˆ Î”Ë¡ a â†‘ (ÏÎµ Î³)

    ÏÎ”Ë¡Îµ-lem 0T = P.â‰ˆ-refl
    ÏÎ”Ë¡Îµ-lem (var y) = P.â‰ˆ-refl
    ÏÎ”Ë¡Îµ-lem (var z) = P.â‰ˆ-refl
    ÏÎ”Ë¡Îµ-lem (c [Â·] Î³) = {!   !}
    ÏÎ”Ë¡Îµ-lem (Î³ [+] Î´) = {!   !}
    ÏÎ”Ë¡Îµ-lem (Î³ [*] Î´) = {!   !}

    -- assume
    -- Î”Ê³ b â†‘ (Î”Ë¡ a â†‘ Î³) Pâ‰ˆ Î”Ë¡ a â†‘ (Î”Ê³ b â†‘ Î³)
    -- and show
    -- Î”Ê³a (Î”Ë¡Îµ Î³) Pâ‰ˆ Î”Ë¡b (Î”Ê³Îµ Î³)

    -- can show Ïab (Î”Ê³a (Î”Ë¡Îµ Î³)) Pâ‰ˆ Ïab (Î”Ë¡b (Î”Ê³Îµ Î³)) :

    -- Ïab (Î”Ê³a (Î”Ë¡Îµ Î³))
    -- Î”Ê³ b â†‘ (Ïa (Î”Ë¡Îµ Î³))
    -- Î”Ê³ b â†‘ (Î”Ë¡ a â†‘ (ÏÎµ Î³))
    -- Î”Ë¡ a â†‘ (Î”Ê³ b â†‘ (ÏÎµ Î³))
    -- Î”Ë¡ a â†‘ (Ïb (Î”Ê³Îµ Î³))
    -- Ïab (Î”Ë¡b (Î”Ê³Îµ Î³))

    -- Î”Ê³a (Î”Ë¡Îµ Î³) Pâ‰ˆ
    -- Î”Ë¡b (Î”Ê³Îµ Î³)

```

```
module _ (special : Special P) where

    open import Special.Automata R Î£ P special

    Î”Ê³Î”Ë¡â†’âŸ¦Î”Ê³Î”Ë¡âŸ§ : Î”Ê³Î”Ë¡ â†’ âŸ¦Î”Ê³Î”Ë¡âŸ§
    Î”Ê³Î”Ë¡â†’âŸ¦Î”Ê³Î”Ë¡âŸ§ ass a b Î± = semantic-invariance S (ass a b Î±)

    Î”Ê³Î”Ë¡-varâ†’Î”Ê³Î”Ë¡ : Î”Ê³Î”Ë¡-var â†’ Î”Ê³Î”Ë¡
    Î”Ê³Î”Ë¡-varâ†’Î”Ê³Î”Ë¡ ass-var a b = go where

        go : âˆ€ Î± â†’ Î”Ê³ b â†‘ (Î”Ë¡ a â†‘ Î±) Pâ‰ˆ Î”Ë¡ a â†‘ (Î”Ê³ b â†‘ Î±)
        go 0T = P.â‰ˆ-refl
        go (var (_ x[ _ ] _)) = P.â‰ˆ-refl
        go (c [Â·] Î±) with go Î±
        ... | ind = P.Â·-cong R-refl ind
        go (Î± [+] Î²) with go Î± | go Î²
        ... | indâ‚€ | indâ‚ = indâ‚€ âŸ¨ P.+-cong âŸ© indâ‚
        go (Î± [*] Î²) with go Î± | go Î²
        ... | indâ‚€ | indâ‚ = proof where

            open Assumptions a b

            -- Îµâ†’ab : Term ÎµXÎµ â†’ Term aXb
            -- Îµâ†’ab 0T = 0T
            -- Îµâ†’ab (var y) = var y
            -- Îµâ†’ab (var z) = var z
            -- Îµâ†’ab (c [Â·] u) = c [Â·] Îµâ†’ab u
            -- Îµâ†’ab (u [+] v) = Îµâ†’ab u [+] Îµâ†’ab v
            -- Îµâ†’ab (u [*] v) = Îµâ†’ab u [*] Îµâ†’ab v

            Ï-Îµ : Subst ÎµXÎµ *X*
            Ï-Îµ y = Î±
            Ï-Îµ z = Î²

            Ï-a : Subst aX *X*
            Ï-a y = Î±
            Ï-a ay = Î”Ë¡ a â†‘ Î±
            Ï-a z = Î²
            Ï-a az = Î”Ë¡ a â†‘ Î²

            Ï-b : Subst Xb *X*
            Ï-b y = Î±
            Ï-b yb = Î”Ê³ b â†‘ Î±
            Ï-b z = Î²
            Ï-b zb = Î”Ê³ b â†‘ Î²

            Ï-ab : Subst aXb *X*
            Ï-ab y = Î±
            Ï-ab ay = Î”Ë¡ a â†‘ Î±
            Ï-ab yb = Î”Ê³ b â†‘ Î±
            Ï-ab ayb = Î”Ê³ b â†‘ (Î”Ë¡ a â†‘ Î±)
            Ï-ab z = Î²
            Ï-ab az = Î”Ë¡ a â†‘ Î²
            Ï-ab zb = Î”Ê³ b â†‘ Î²
            Ï-ab azb = Î”Ê³ b â†‘ (Î”Ë¡ a â†‘ Î²)

            h-a :
                (Î³ : Term ÎµXÎµ) â†’
                --------------------------------
                subst Ï-Îµ Î³ Pâ‰ˆ subst Ï-a (Îµâ†’a Î³)
                
            h-a 0T = P.â‰ˆ-refl
            h-a (var y) = P.â‰ˆ-refl
            h-a (var z) = P.â‰ˆ-refl
            h-a (c [Â·] Î³) = R-refl âŸ¨ P.Â·-cong âŸ© h-a Î³
            h-a (Î³ [+] Î´) = h-a Î³ âŸ¨ P.+-cong âŸ© h-a Î´
            h-a (Î³ [*] Î´) = h-a Î³ âŸ¨ P.*-cong âŸ© h-a Î´

            h-b :
                (Î³ : Term ÎµXÎµ) â†’
                --------------------------------
                subst Ï-Îµ Î³ Pâ‰ˆ subst Ï-b (Îµâ†’b Î³)
                
            h-b 0T = P.â‰ˆ-refl
            h-b (var y) = P.â‰ˆ-refl
            h-b (var z) = P.â‰ˆ-refl
            h-b (c [Â·] Î³) = R-refl âŸ¨ P.Â·-cong âŸ© h-b Î³
            h-b (Î³ [+] Î´) = h-b Î³ âŸ¨ P.+-cong âŸ© h-b Î´
            h-b (Î³ [*] Î´) = h-b Î³ âŸ¨ P.*-cong âŸ© h-b Î´

            subst-bâ†’ab :
                (Î³ : Term Xb) â†’
                --------------------------------
                subst Ï-b Î³ Pâ‰ˆ subst Ï-ab (bâ†’ab Î³)
                
            subst-bâ†’ab 0T = P.â‰ˆ-refl
            subst-bâ†’ab (var y) = P.â‰ˆ-refl
            subst-bâ†’ab (var yb) = P.â‰ˆ-refl
            subst-bâ†’ab (var z) = P.â‰ˆ-refl
            subst-bâ†’ab (var zb) = P.â‰ˆ-refl
            subst-bâ†’ab (c [Â·] Î³) = R-refl âŸ¨ P.Â·-cong âŸ© subst-bâ†’ab Î³
            subst-bâ†’ab (Î³ [+] Î´) = subst-bâ†’ab Î³ âŸ¨ P.+-cong âŸ© subst-bâ†’ab Î´
            subst-bâ†’ab (Î³ [*] Î´) = subst-bâ†’ab Î³ âŸ¨ P.*-cong âŸ© subst-bâ†’ab Î´

            subst-aâ†’ab :
                (Î³ : Term aX) â†’
                --------------------------------
                subst Ï-a Î³ Pâ‰ˆ subst Ï-ab (aâ†’ab Î³)
                
            subst-aâ†’ab 0T = P.â‰ˆ-refl
            subst-aâ†’ab (var y) = P.â‰ˆ-refl
            subst-aâ†’ab (var ay) = P.â‰ˆ-refl
            subst-aâ†’ab (var z) = P.â‰ˆ-refl
            subst-aâ†’ab (var az) = P.â‰ˆ-refl
            subst-aâ†’ab (c [Â·] Î³) = R-refl âŸ¨ P.Â·-cong âŸ© subst-aâ†’ab Î³
            subst-aâ†’ab (Î³ [+] Î´) = subst-aâ†’ab Î³ âŸ¨ P.+-cong âŸ© subst-aâ†’ab Î´
            subst-aâ†’ab (Î³ [*] Î´) = subst-aâ†’ab Î³ âŸ¨ P.*-cong âŸ© subst-aâ†’ab Î´

            Î”Ë¡Îµ-lem :
                (Î³ : Term ÎµXÎµ) â†’
                ---------------------------------------
                Î”Ë¡ a â†‘ subst Ï-Îµ Î³ Pâ‰ˆ subst Ï-a (Î”Ë¡Îµ Î³)

            Î”Ë¡Îµ-lem 0T = P.â‰ˆ-refl
            Î”Ë¡Îµ-lem (var y) = P.â‰ˆ-refl
            Î”Ë¡Îµ-lem (var z) = P.â‰ˆ-refl
            Î”Ë¡Îµ-lem (c [Â·] Î³) = R-refl âŸ¨ P.Â·-cong âŸ© Î”Ë¡Îµ-lem Î³
            Î”Ë¡Îµ-lem (Î³ [+] Î´) = Î”Ë¡Îµ-lem Î³ âŸ¨ P.+-cong âŸ© Î”Ë¡Îµ-lem Î´
            Î”Ë¡Îµ-lem (Î³ [*] Î´) =
                begin
                    Î”Ë¡ a â†‘ subst Ï-Îµ (Î³ [*] Î´)
                        â‰ˆâŸ¨âŸ©
                    [ P ]âŸ¨ subst Ï-Îµ Î³ , Î”Ë¡ a â†‘ subst Ï-Îµ Î³ , subst Ï-Îµ Î´ , Î”Ë¡ a â†‘ subst Ï-Îµ Î´ âŸ©
                        â‰ˆâŸ¨ subst-invâ€²áµ¥ P (h-a Î³ âˆ·-â‰ˆ Î”Ë¡Îµ-lem Î³ âˆ·-â‰ˆ h-a Î´ âˆ·-â‰ˆ Î”Ë¡Îµ-lem Î´ âˆ·-â‰ˆ []-â‰ˆ) âŸ©
                    [ P ]âŸ¨ subst Ï-a (Îµâ†’a Î³) , subst Ï-a (Î”Ë¡Îµ Î³) , subst Ï-a (Îµâ†’a Î´) , subst Ï-a (Î”Ë¡Îµ Î´) âŸ©
                        â‰¡âŸ¨ subst-substáµ¥ P (_ âˆ· _ âˆ· _ âˆ· _ âˆ· []) Ï-a âŸ¨
                    subst Ï-a [ P ]âŸ¨ Îµâ†’a Î³ , Î”Ë¡Îµ Î³ , Îµâ†’a Î´ , Î”Ë¡Îµ Î´ âŸ©
                âˆ where open EqP

            Î”Ê³Îµ-lem :
                âˆ€ (Î³ : Term ÎµXÎµ) â†’
                ---------------------------------
                Î”Ê³ b â†‘ (subst Ï-Îµ Î³) Pâ‰ˆ subst Ï-b (Î”Ê³Îµ Î³)

            Î”Ê³Îµ-lem 0T = P.â‰ˆ-refl
            Î”Ê³Îµ-lem (var y) = P.â‰ˆ-refl
            Î”Ê³Îµ-lem (var z) = P.â‰ˆ-refl
            Î”Ê³Îµ-lem (c [Â·] Î³) = R-refl âŸ¨ P.Â·-cong âŸ© Î”Ê³Îµ-lem Î³
            Î”Ê³Îµ-lem (Î³ [+] Î´) = Î”Ê³Îµ-lem Î³ âŸ¨ P.+-cong âŸ© Î”Ê³Îµ-lem Î´
            Î”Ê³Îµ-lem (Î³ [*] Î´) =
                begin
                    Î”Ê³ b â†‘ subst Ï-Îµ (Î³ [*] Î´)
                        â‰ˆâŸ¨âŸ©
                    [ P ]âŸ¨ subst Ï-Îµ Î³ , Î”Ê³ b â†‘ subst Ï-Îµ Î³ , subst Ï-Îµ Î´ , Î”Ê³ b â†‘ subst Ï-Îµ Î´ âŸ©
                        â‰ˆâŸ¨ subst-invâ€²áµ¥ P (h-b Î³ âˆ·-â‰ˆ Î”Ê³Îµ-lem Î³ âˆ·-â‰ˆ h-b Î´ âˆ·-â‰ˆ Î”Ê³Îµ-lem Î´ âˆ·-â‰ˆ []-â‰ˆ) âŸ©
                    [ P ]âŸ¨ subst Ï-b (Îµâ†’b Î³) , subst Ï-b (Î”Ê³Îµ Î³) , subst Ï-b (Îµâ†’b Î´) , subst Ï-b (Î”Ê³Îµ Î´) âŸ©
                        â‰¡âŸ¨ subst-substáµ¥ P (_ âˆ· _ âˆ· _ âˆ· _ âˆ· []) Ï-b âŸ¨
                    subst Ï-b (Î”Ê³Îµ (Î³ [*] Î´))
                âˆ where open EqP

            Î”Ë¡b-lem :
                âˆ€ (Î³ : Term Xb) â†’
                ---------------------------------
                Î”Ë¡ a â†‘ (subst Ï-b Î³) Pâ‰ˆ subst Ï-ab (Î”Ë¡b Î³)

            Î”Ë¡b-lem 0T = P.â‰ˆ-refl
            Î”Ë¡b-lem (var y) = P.â‰ˆ-refl
            Î”Ë¡b-lem (var yb) = P.â‰ˆ-sym indâ‚€
            Î”Ë¡b-lem (var z) = P.â‰ˆ-refl
            Î”Ë¡b-lem (var zb) = P.â‰ˆ-sym indâ‚
            Î”Ë¡b-lem (c [Â·] Î³) = R-refl âŸ¨ P.Â·-cong âŸ© Î”Ë¡b-lem Î³
            Î”Ë¡b-lem (Î³ [+] Î´) = Î”Ë¡b-lem Î³ âŸ¨ P.+-cong âŸ© Î”Ë¡b-lem Î´
            Î”Ë¡b-lem (Î³ [*] Î´) =
                begin
                    Î”Ë¡ a â†‘ subst Ï-b (Î³ [*] Î´)
                        â‰ˆâŸ¨âŸ©
                    [ P ]âŸ¨ subst Ï-b Î³ , Î”Ë¡ a â†‘ subst Ï-b Î³ , subst Ï-b Î´ , Î”Ë¡ a â†‘ subst Ï-b Î´ âŸ©
                        â‰ˆâŸ¨ subst-invâ€²áµ¥ P (subst-bâ†’ab Î³ âˆ·-â‰ˆ Î”Ë¡b-lem Î³ âˆ·-â‰ˆ subst-bâ†’ab Î´ âˆ·-â‰ˆ Î”Ë¡b-lem Î´ âˆ·-â‰ˆ []-â‰ˆ) âŸ©
                    [ P ]âŸ¨ subst Ï-ab (bâ†’ab Î³) , subst Ï-ab (Î”Ë¡b Î³) , subst Ï-ab (bâ†’ab Î´) , subst Ï-ab (Î”Ë¡b Î´) âŸ©
                        â‰¡âŸ¨ subst-substáµ¥ P (_ âˆ· _ âˆ· _ âˆ· _ âˆ· []) Ï-ab âŸ¨
                    subst Ï-ab (Î”Ë¡b (Î³ [*] Î´))
                âˆ where open EqP

            Î”Ê³a-lem :
                âˆ€ (Î³ : Term aX) â†’
                ---------------------------------
                Î”Ê³ b â†‘ (subst Ï-a Î³) Pâ‰ˆ subst Ï-ab (Î”Ê³a Î³)

            Î”Ê³a-lem 0T = P.â‰ˆ-refl
            Î”Ê³a-lem (var y) = P.â‰ˆ-refl
            Î”Ê³a-lem (var ay) = P.â‰ˆ-refl
            Î”Ê³a-lem (var z) = P.â‰ˆ-refl
            Î”Ê³a-lem (var az) = P.â‰ˆ-refl
            Î”Ê³a-lem (c [Â·] Î³) = R-refl âŸ¨ P.Â·-cong âŸ© Î”Ê³a-lem Î³
            Î”Ê³a-lem (Î³ [+] Î´) = Î”Ê³a-lem Î³ âŸ¨ P.+-cong âŸ© Î”Ê³a-lem Î´
            Î”Ê³a-lem (Î³ [*] Î´) =
                begin
                    Î”Ê³ b â†‘ subst Ï-a (Î³ [*] Î´)
                        â‰ˆâŸ¨âŸ©
                    [ P ]âŸ¨ subst Ï-a Î³ , Î”Ê³ b â†‘ subst Ï-a Î³ , subst Ï-a Î´ , Î”Ê³ b â†‘ subst Ï-a Î´ âŸ©
                        â‰ˆâŸ¨ subst-invâ€²áµ¥ P (subst-aâ†’ab Î³ âˆ·-â‰ˆ Î”Ê³a-lem Î³ âˆ·-â‰ˆ subst-aâ†’ab Î´ âˆ·-â‰ˆ Î”Ê³a-lem Î´ âˆ·-â‰ˆ []-â‰ˆ) âŸ©
                    [ P ]âŸ¨ subst Ï-ab (aâ†’ab Î³) , subst Ï-ab (Î”Ê³a Î³) , subst Ï-ab (aâ†’ab Î´) , subst Ï-ab (Î”Ê³a Î´) âŸ©
                        â‰¡âŸ¨ subst-substáµ¥ P (_ âˆ· _ âˆ· _ âˆ· _ âˆ· []) Ï-ab âŸ¨
                    subst Ï-ab (Î”Ê³a (Î³ [*] Î´))
                âˆ where open EqP

            proof : Î”Ê³ b â†‘ (Î”Ë¡ a â†‘ (Î± [*] Î²)) Pâ‰ˆ Î”Ë¡ a â†‘ (Î”Ê³ b â†‘ (Î± [*] Î²))
            proof =
                begin
                    Î”Ê³ b â†‘ (Î”Ë¡ a â†‘ (Î± [*] Î²))
                        â‰ˆâŸ¨âŸ©
                    Î”Ê³ b â†‘ (Î”Ë¡ a â†‘ (subst Ï-Îµ (var y [*] var z)))
                        â‰ˆâŸ¨ invariance (Î”Ê³ b) (Î”Ë¡Îµ-lem (var y [*] var z)) âŸ©
                    Î”Ê³ b â†‘ (subst Ï-a (Î”Ë¡Îµ (var y [*] var z)))
                        â‰ˆâŸ¨ Î”Ê³a-lem (Î”Ë¡Îµ (var y [*] var z)) âŸ©
                    subst Ï-ab (Î”Ê³a (Î”Ë¡Îµ (var y [*] var z)))
                        â‰ˆâŸ¨ subst-inv Ï-ab (ass-var a b) âŸ©
                    subst Ï-ab (Î”Ë¡b (Î”Ê³Îµ (var y [*] var z)))
                        â‰ˆâŸ¨ Î”Ë¡b-lem (Î”Ê³Îµ (var y [*] var z)) âŸ¨
                    Î”Ë¡ a â†‘ (subst Ï-b (Î”Ê³Îµ (var y [*] var z)))
                        â‰ˆâŸ¨ invariance (Î”Ë¡ a) (Î”Ê³Îµ-lem (var y [*] var z)) âŸ¨
                    Î”Ë¡ a â†‘ (Î”Ê³ b â†‘ (subst Ï-Îµ (var y [*] var z)))
                        â‰ˆâŸ¨âŸ©
                    Î”Ë¡ a â†‘ (Î”Ê³ b â†‘ (Î± [*] Î²))
                âˆ where open EqP

```


