---
title: ðŸš§
---

```
open import Preliminaries.Base
import Preliminaries.Algebra

module Preliminaries.PolyExpr.Integer (R : CommutativeRing)
    where

open import Algebra

open CommutativeRing R renaming
    (Carrier to CarrierR;
    0# to 0R;
    1# to 1R;
    _+_ to _+R_;
    -_ to -R_;
    _*_ to _*R_;
    _â‰ˆ_ to _â‰ˆR_;
    refl to R-refl;
    sym to R-sym;
    +-cong to +R-cong;
    +-assoc to +R-assoc;
    +-identityË¡ to +R-identityË¡;
    *-identityË¡ to *R-identityË¡;
    zeroË¡ to R-zeroË¡;
    distribË¡ to R-distribË¡;
    distribÊ³ to R-distribÊ³;
    isEquivalence to isEquivalenceR
    )

open import Preliminaries.Equivalence isEquivalenceR

open import Data.Nat.Base as â„•
    using (â„•; suc; zero)
    renaming (_+_ to _+â„•_; _*_ to _*â„•_)
    
import Data.Nat.Properties as â„•

open import Data.Integer.Base as â„¤ using (â„¤; +_)
open import Data.Integer.Properties as â„¤

open import Preliminaries.PolyExpr.Homomorphism -- â„¤.+-*-commutativeRing R
```

The integers map homomorphically to every commutative ring.

```
Ï†â„• : â„• â†’ CarrierR
Ï†â„• zero = 0R
Ï†â„• (suc n) = 1R +R Ï†â„• n

Ï†â„¤ : â„¤ â†’ CarrierR
Ï†â„¤ (+ n) = Ï†â„• n
Ï†â„¤ (â„¤.-[1+ n ]) = -R (1R +R Ï†â„• n)

open CommutativeRing â„¤.+-*-commutativeRing

â‰ˆ-hom-Ï†â„¤ : âˆ€ {a b} â†’ a â‰¡ b â†’ Ï†â„¤ a â‰ˆR Ï†â„¤ b
â‰ˆ-hom-Ï†â„¤ refl = R-refl

1+0â‰ˆ1 : 1R +R 0R â‰ˆR 1R
1+0â‰ˆ1 = {!   !}

+-hom-Ï†â„• : âˆ€ a b â†’ Ï†â„• (a +â„• b) â‰ˆR Ï†â„• a +R Ï†â„• b
+-hom-Ï†â„• zero b = R-sym (+R-identityË¡ _)
+-hom-Ï†â„• (suc a) b = 
    begin
        1R +R Ï†â„• (a +â„• b)
            â‰ˆâŸ¨ +R-cong R-refl (+-hom-Ï†â„• a b) âŸ©
        1R +R (Ï†â„• a +R Ï†â„• b)
            â‰ˆâŸ¨ +R-assoc _ _ _ âŸ¨
        1R +R Ï†â„• a +R Ï†â„• b
    âˆŽ where open Eq

*-hom-Ï†â„• : âˆ€ a b â†’ Ï†â„• (a *â„• b) â‰ˆR Ï†â„• a *R Ï†â„• b
*-hom-Ï†â„• zero b = R-sym (R-zeroË¡ _)
*-hom-Ï†â„• (suc a) b =
    begin
        Ï†â„• (b +â„• a *â„• b)
            â‰ˆâŸ¨ +-hom-Ï†â„• b _ âŸ©
        Ï†â„• b +R Ï†â„• (a *â„• b)
            â‰ˆâŸ¨ R-refl âŸ¨ +R-cong âŸ© *-hom-Ï†â„• a b âŸ©
        Ï†â„• b +R (Ï†â„• a *R Ï†â„• b)
            â‰ˆâŸ¨  *R-identityË¡ _ âŸ¨ +R-cong âŸ© R-refl âŸ¨
        (1R *R Ï†â„• b) +R (Ï†â„• a *R Ï†â„• b)
            â‰ˆâŸ¨ R-distribÊ³ _ _ _ âŸ¨
        (1R +R Ï†â„• a) *R Ï†â„• b
    âˆŽ where open Eq

+-hom-Ï†â„¤ : âˆ€ a b â†’ Ï†â„¤ (a + b) â‰ˆR Ï†â„¤ a +R Ï†â„¤ b
+-hom-Ï†â„¤ (+ n) (+ m) = +-hom-Ï†â„• n m
+-hom-Ï†â„¤ (+_ n) (â„¤.-[1+_] m) = {!   !}
+-hom-Ï†â„¤ (â„¤.-[1+_] n) b = {!   !}

*-hom-Ï†â„¤ : âˆ€ a b â†’ Ï†â„¤ (a * b) â‰ˆR Ï†â„¤ a *R Ï†â„¤ b
*-hom-Ï†â„¤ = {!   !}

Ï†â„¤-isRingHom : IsRingHom â„¤.+-*-commutativeRing R Ï†â„¤
Ï†â„¤-isRingHom = record
  { â‰ˆ-hom = â‰ˆ-hom-Ï†â„¤
  ; 0-hom = R-refl
  ; 1-hom = 1+0â‰ˆ1
  ; +-hom = +-hom-Ï†â„¤
  ; *-hom = *-hom-Ï†â„¤ }
```